PHeap.v
@@ -1,0 +1,317 @@
+Require Import Logic.Eqdep.
+Require Import Bool.
+Require Import Arith.
+Require Import ZArith.
+Require Import String.
+Require Import QArith.
+Require Import Qcanon.
+Require Import Coq.Relations.Relations.
+
+Require ClassicalFacts.
+Require Export FunctionalExtensionality.
+Require Export ProofIrrelevance.
+
+Require Export Coq.ZArith.BinInt.
+Require Export String.
+
+Add LoadPath "../../src/cslsound".
+
+Require Export Vbase Varith Vlistbase Vlist Basic.
+
+Set Implicit Arguments.
+Unset Strict Implicit.
+
+Definition pheap' := Z -> option (Qc * Z).
+
+Definition is_pheap (h : pheap') : Prop :=
+  forall x, match h x with
+    | None => True
+    | Some (p, v) => 0 < p /\ p <= 1
+  end.
+Record pheap := Pheap { this :> pheap'; is_p : is_pheap this }.
+Definition pdisj (h1 h2 : pheap') :=
+  forall (x : Z), match h1 x, h2 x with
+    | None, _ | _, None => True
+    | Some (p1, v1), some (p2, v2) =>
+      v1 = v2 /\ 0 < p1 + p2 /\ p1 + p2 <= 1
+  end.
+
+Definition phplus (h1 h2 : pheap') : pheap' :=
+  fun x => match h1 x with
+    | None => h2 x
+    | Some (p1, v1) => 
+      match h2 x with
+        | None => h1 x
+        | Some (p2, v2) => Some (p1 + p2, v1)
+      end
+  end.
+
+Definition full_p : Qc := 1.
+Definition emp_h : pheap' := fun (n : Z) => None.
+
+Definition fpdom (h : pheap') : Prop :=
+  forall (n : Z), match h n with
+    | None => True
+    | Some (p, v) => (p = full_p)%Qc
+  end.
+
+Lemma pdisjC : forall h1 h2, pdisj h1 h2 -> pdisj h2 h1.
+Proof. 
+  unfold pdisj, pheap'; intros h1 h2 hd x.
+  specialize (hd x).
+  destruct (h1 x), (h2 x); try tauto.
+  destruct p as [? ?], p0 as [? ?].
+  assert (q0 + q = q + q0) as heq by ring; rewrite heq.
+  destruct hd as [? [? ?]]; repeat split; auto.
+Qed.
+
+Lemma pdisj_empty1 : forall (h : pheap), pdisj emp_h h.
+  intros h; unfold emp_h, pdisj; simpl; eauto.
+Qed.
+
+Lemma pdisj_empty2 : forall (h : pheap), pdisj h emp_h.
+  now unfold emp_h, pdisj; intros h x; destruct (this h x) as [[? ?] | ?].
+Qed.
+
+Definition ph_upd (h : pheap') (x : Z) (v : Z) : pheap' :=
+  fun (x' : Z) => if Z.eq_dec x x' then Some (full_p, v) else h x'.
+
+Lemma ph_upd_ph (h : pheap) (x : Z) (v : Z) : is_pheap (ph_upd h x v).
+Proof.
+  destruct h as [h ph]; simpl.
+  unfold is_pheap, ph_upd; intros y; destruct (Z.eq_dec x y).
+  - split; unfold Qclt, Qlt, Qcle, Qle, full_p; simpl; omega.
+  - specialize (ph y); eauto.
+Qed.
+
+Definition ph_upd2 (h : pheap) (x : Z) (v : Z) : pheap :=
+  @Pheap (ph_upd h x v) (ph_upd_ph h x v).
+
+Definition empty_p := 0.
+
+Lemma frac_contra1 : forall p : Qc, (p > empty_p)%Qc -> ~(full_p + p <= full_p)%Qc.
+Proof.
+  unfold full_p; intros p hp hcontra.
+  apply (Qcle_minus_iff (1 + p) 1) in hcontra.
+  assert (1 + - (1 + p) = -p) as h by ring; rewrite h in hcontra; clear h.
+  apply Qcopp_le_compat in hcontra.
+  assert (- -p = p) as h by ring; rewrite h in hcontra; clear h.
+  assert (- 0 = 0) as h by ring; rewrite h in hcontra; clear h.
+  apply Qclt_not_le in hp; tauto.
+Qed.
+
+Lemma frac_contra2 : forall p, p > empty_p -> ~(p + full_p <= 1).
+Proof.
+  intros ? ?; rewrite Qcplus_comm.
+  auto using frac_contra1.
+Qed.
+
+Lemma pdisj_upd : forall (h h' : pheap) (x w v : Z), this h x = Some (full_p, w) -> 
+  (pdisj (ph_upd h x v) h' <-> pdisj h h').
+Proof.
+  destruct h as [h iph].
+  destruct h' as [h' iph'].
+  unfold pdisj, ph_upd; ins.
+  split. 
+  - intros hp x0; pose proof (hp x0); pose proof (iph x0); pose proof (iph' x0).
+    destruct (Z.eq_dec x x0), (h x0) as [[? ?] | ], (h' x0) as [[? ?] | ]; eauto.
+    destruct H0 as [? [? ?]],  H2 as [? ?]; exfalso; eapply (@frac_contra1 q0); eauto.
+  - intros hp x0; specialize (hp x0); specialize (iph x0); specialize (iph' x0).
+    destruct (Z.eq_dec x x0); subst;
+    destruct (h x0) as [[? ?] | ], (h' x0) as [[? ?] | ]; simpl; eauto;
+    inversion H; subst.
+    destruct hp as [? [? ?]], iph' as [? ?]; exfalso; eapply (@frac_contra1 q0); eauto.
+Qed.
+
+Lemma phplus_comm (h1 h2 : pheap) : pdisj h1 h2 -> phplus h1 h2 = phplus h2 h1.
+Proof.
+  destruct h1 as [h1 H1], h2 as [h2 H2]; simpl.
+  intros hdisj; unfold is_pheap, pdisj, phplus in *; extensionality x.
+  repeat (match goal with [H : forall _ : Z, _ |- _] => specialize (H x) end).
+  destruct (h1 x) as [[? ?] | ], (h2 x) as [[? ?] | ]; eauto. 
+  destruct hdisj as [? [? ?]].
+  assert (q + q0 = q0 + q) by ring; congruence.
+Qed.
+
+Lemma plus_gt_0 : forall p1 p2 : Qc, 0 < p1 -> 0 < p2 -> 0 < p1 + p2.
+Proof.
+  intros p1 p2 h1 h2.
+  assert (p2 < p1 + p2).
+  { apply Qclt_minus_iff.
+    cutrewrite (p1 + p2 + - p2 = p1); [eauto | ring]. }
+  apply (Qclt_trans _ p2 _); eauto.
+Qed.
+
+Lemma gt_0_plus : forall p p1 : Qc, 0 < p1 -> p < p + p1.
+Proof.
+  intros p p1 h1.
+  apply Qclt_minus_iff.
+  cutrewrite (p + p1 + - p = p1); [eauto | ring].
+Qed.
+
+Lemma le1_weak : forall p p1 : Qc, 0 < p1 -> p + p1 <= 1 -> p <= 1.
+Proof.
+  intros p p1 h1 hp.
+  apply Qclt_le_weak.
+  apply (Qclt_le_trans _ (p + p1) _); [apply gt_0_plus; eauto | eauto].
+Qed.
+
+Lemma pdisj_padd (h1 h2 h3 : pheap) :
+  pdisj h2 h3 -> pdisj h1 (phplus h2 h3) -> (pdisj h1 h2) /\ (pdisj h1 h3).
+Proof.
+  destruct h1 as [h1 H1], h2 as [h2 H2], h3 as [h3 H3]; simpl.
+  unfold is_pheap, pdisj, phplus in *;
+    intros disj23 disj123; split; intros x; 
+    repeat (match goal with [H : forall _ : Z, _ |- _] => specialize (H x) end);
+    destruct (h1 x) as [[? ?] |], (h2 x) as [[? ?] |], (h3 x) as [[? ?] |];
+    destruct disj23 as [? [? ?]], disj123 as [? [? ?]], H1 as [? ?], H2 as [? ?], H3 as [? ?];
+    repeat split; eauto using Qcplus_comm.
+
+  - apply plus_gt_0; eauto.
+  - cutrewrite (q + (q0 + q1) = (q + q0) + q1) in H7; [apply (@le1_weak _ q1); eauto | ring ].
+  - congruence.
+  - apply plus_gt_0; eauto.
+  - cutrewrite (q + (q0 + q1) = (q + q1) + q0) in H7; [apply (@le1_weak _ q0); eauto | ring ].
+Qed.
+
+Lemma pdisjE1 (h1 h2 h3 : pheap) : pdisj h1 (phplus h2 h3) -> pdisj h2 h3 -> pdisj h1 h2.
+Proof.
+  destruct h1 as [h1 ph1], h2 as [h2 ph2], h3 as [h3 ph3]; simpl in *.
+  unfold is_pheap, pdisj, phplus in *;
+    intros h123 h23 x;
+    repeat (match goal with [H : forall _ : Z, _ |- _] => specialize (H x) end).
+  destruct (h1 x) as [[? ?] |], (h2 x) as [[? ?] |], (h3 x) as [[? ?] |],
+                                                               ph1 as [? ?], ph2 as [? ?], ph3 as [? ?], h123 as [? [? ?]], h23 as [? [? ?]]; eauto.
+  repeat split; eauto using plus_gt_0.
+  cutrewrite (q + (q0 + q1) = (q + q0) + q1) in H7; [apply (@le1_weak _ q1); eauto | ring ].
+Qed.
+
+Lemma pdisjE2 (h1 h2 h3 : pheap) :
+  pdisj h1 (phplus h2 h3) -> pdisj h2 h3 -> pdisj h1 h3.
+Proof.
+  destruct h1 as [h1 ph1], h2 as [h2 ph2], h3 as [h3 ph3]; simpl in *.
+  unfold is_pheap, pdisj, phplus in *;
+    intros h123 h23 x;
+    repeat (match goal with [H : forall _ : Z, _ |- _] => specialize (H x) end).
+  destruct (h1 x) as [[? ?] |], (h2 x) as [[? ?] |], (h3 x) as [[? ?] |],
+                                                               ph1 as [? ?], ph2 as [? ?], ph3 as [? ?], h123 as [? [? ?]], h23 as [? [? ?]]; eauto.
+  repeat split; eauto using plus_gt_0.
+  - congruence.
+  - cutrewrite (q + (q0 + q1) = (q + q1) + q0) in H7; [apply (@le1_weak _ q0); eauto | ring ].
+Qed.
+
+Lemma pdisj_padd_comm (h1 h2 h3 : pheap) : pdisj h2 (phplus h1 h3) -> pdisj h1 h3 -> 
+                                           pdisj h1 (phplus h2 h3).
+Proof.
+  destruct h1 as [h1 ph1], h2 as [h2 ph2], h3 as [h3 ph3]; simpl in *.
+  unfold is_pheap, pdisj, phplus in *;
+    intros h123 h23 x;
+    repeat (match goal with [H : forall _ : Z, _ |- _] => specialize (H x) end).
+  destruct (h1 x) as [[? ?] |], (h2 x) as [[? ?] |], (h3 x) as [[? ?] |],
+    ph1 as [? ?], ph2 as [? ?], ph3 as [? ?], h123 as [? [? ?]], h23 as [? [? ?]]; eauto.
+  - cutrewrite (q + (q0 + q1) = q0 + (q + q1)); [ | ring].
+    repeat split; eauto.
+  - cutrewrite (q + q0 = q0 + q); [ | ring];
+    repeat split; eauto.
+Qed.
+
+Lemma pdisj_padd_expand (h1 h2 h3 : pheap) : 
+  pdisj h1 h2 -> (pdisj (phplus h1 h2) h3 <-> (pdisj h1 (phplus h2 h3) /\ pdisj h2 h3)).
+Proof.
+  destruct h1 as [h1 ph1], h2 as [h2 ph2], h3 as [h3 ph3]; simpl in *.
+  unfold is_pheap, pdisj, phplus in *;
+    intros h12; split; [intros H; split; intros x | intros [H1 H2] x];
+    repeat (match goal with [H : forall _ : Z, _ |- _] => specialize (H x) end);
+    destruct (h1 x) as [[? ?] |], (h2 x) as [[? ?] |], (h3 x) as [[? ?] |],
+                                                                 ph1 as [? ?], ph2 as [? ?], ph3 as [? ?], h12 as [? [? ?]];
+    des; eauto;
+    repeat split; try congruence; eauto; 
+    try rewrite (Qcplus_assoc _ _ _); try rewrite (Qcplus_comm _ _); 
+    eauto using plus_gt_0.
+  - cutrewrite (q1 + (q + q0) = q + q0 + q1); [eauto | ring].
+  - cutrewrite (q + q0 + q1 = (q1 + q0) + q) in H10; [apply (@le1_weak _ q); eauto | ring].
+  - cutrewrite (q1 + (q + q0) = q + (q0 + q1)); [eauto | ring].
+Qed.
+
+Lemma padd_assoc (h1 h2 h3 : pheap) :
+  pdisj h1 (phplus h2 h3) -> pdisj h2 h3 -> phplus (phplus h1 h2) h3 = phplus h1 (phplus h2 h3).
+Proof.
+  destruct h1 as [h1 ph1], h2 as [h2 ph2], h3 as [h3 ph3]; simpl in *.
+  unfold is_pheap, pdisj, phplus in *;
+    intros h123 h23; extensionality x;
+    repeat (match goal with [H : forall _ : Z, _ |- _] => specialize (H x) end);
+    destruct (h1 x) as [[? ?] |], (h2 x) as [[? ?] |], (h3 x) as [[? ?] |];
+    des; eauto.
+  cutrewrite (q + q0 + q1 = q + (q0 + q1)); [eauto | ring].
+Qed.
+
+Lemma padd_left_comm (h1 h2 h3 : pheap) :
+  pdisj h1 (phplus h2 h3) -> pdisj h2 h3 -> phplus h1 (phplus h2 h3) = phplus h2 (phplus h1 h3).
+Proof.
+  destruct h1 as [h1 ph1], h2 as [h2 ph2], h3 as [h3 ph3]; simpl in *.
+  unfold is_pheap, pdisj, phplus in *;
+    intros h123 h23; extensionality x;
+    repeat (match goal with [H : forall _ : Z, _ |- _] => specialize (H x) end);
+    destruct (h1 x) as [[? ?] |], (h2 x) as [[? ?] |], (h3 x) as [[? ?] |];
+    des; eauto.
+  - cutrewrite (q + (q0 + q1) = q0 + (q + q1)); [congruence | ring].
+  - cutrewrite (q + q0 = q0 + q); [congruence | ring].
+Qed.
+
+Lemma padd_cancel (h1 h2 h3 : pheap) :
+  phplus h1 h2 = phplus h1 h3 -> pdisj h1 h2 -> pdisj h1 h3 -> h2 = h3.
+Proof.
+  destruct h1 as [h1 ph1], h2 as [h2 ph2], h3 as [h3 ph3]; simpl in *.
+  intros heq h12 h13.
+  assert (h2 = h3).
+  unfold is_pheap, pdisj, phplus in *;
+    extensionality x; pose proof  (equal_f heq x) as heq'; simpl in *; clear heq;
+    repeat (match goal with [H : forall _ : Z, _ |- _] => specialize (H x) end);
+    destruct (h1 x) as [[? ?] |], (h2 x) as [[? ?] |], (h3 x) as [[? ?] |];
+    des; eauto; try congruence.
+  - remember (q + q0) as q0'; remember (q + q1) as q1'.
+    inversion heq'. subst.
+    assert (q + q0 - q = q + q1 - q) by (rewrite H0; eauto).
+    cutrewrite (q + q0 - q = q0) in H; [| ring].
+    cutrewrite (q + q1 - q = q1) in H; [| ring].
+    congruence.
+  - remember (q + q0) as q'.
+    inversion heq'; subst.
+    assert (q + q0 - q = q - q) by (rewrite H0; eauto).
+    cutrewrite (q + q0 - q = q0) in H; [| ring].
+    cutrewrite (q - q = 0) in H; [| ring].
+    rewrite H in ph2.
+    inversion ph2.
+  - inversion heq'.
+    assert (q - q = (q + q0) - q) by (rewrite H0 at 1; eauto).
+    cutrewrite (q - q = 0) in H; [| ring].
+    cutrewrite (q + q0 - q = q0) in H; [| ring].
+    rewrite <- H in ph3; inversion ph3.
+  - subst; cutrewrite (ph2 = ph3); [eauto | apply proof_irrelevance ].
+Qed.
+
+Corollary padd_cancel2 (h1 h2 h3 : pheap) :
+  phplus h2 h1 = phplus h3 h1 -> pdisj h2 h1 -> pdisj h3 h1 -> h2 = h3.
+Proof.
+  Hint Resolve pdisjC.
+  intros.
+  rewrite (@phplus_comm h2 h1), (@phplus_comm h3 h1) in H; eauto.
+  eapply padd_cancel; eauto.
+Qed.
+
+Definition ptoheap (ph : pheap') (h : heap) : Prop :=
+  forall (x : Z), match ph x with
+                    | None => h x = None
+                    | Some (p, v) => p = full_p /\ h x = Some v
+                  end.
+
+Lemma ptoD (ph1 ph2 : pheap') (h : heap):
+  ptoheap ph1 h -> ptoheap ph2 h -> ph1 = ph2.
+Proof.
+  (*    destruct ph1 as [h1 ph1], ph2 as [h2 ph2]; simpl in *.*)
+  intros pto1 pto2.
+  unfold is_pheap, pdisj, phplus, ptoheap in *; extensionality x; simpl in *;
+  repeat (match goal with [H : forall _ : Z, _ |- _] => specialize (H x) end);
+  destruct (ph1 x) as [[? ?] |], (ph2 x) as [[? ?] |];
+  des; eauto; try congruence.
+Qed.
